Proofs/AES-GCM/GCM.lean
@@ -5,3 +5,4 @@ Author(s): Alex Keizer
 -/
 import Proofs.«AES-GCM».GCMGmultV8Sym
 import Proofs.«AES-GCM».GCMInitV8Sym
+import Proofs.«AES-GCM».AESHWEncryptSym
